
\begin{figure}[H]
\centering

$ J_{OC1}=
\begin{bmatrix}
-\frac{1}{2}s_1l_2    &  &\\
\frac{1}{2}c_1l_2  \\
0 & & \\
0 &\overrightarrow{0} &\overrightarrow{0} \\
0 & &\\
1 & &\\
\end{bmatrix}  
$
\end{figure} 

\begin{figure}[H]
\centering
$ J_{OC2}=
\begin{bmatrix}
-\frac{1}{2}s_1l_2    &c_1  &\\
\frac{1}{2}c_1l_2  & s_1\\
0 &0 & \\
0 &0 &\overrightarrow{0} \\
0 &0 &\\
1 &0 &\\
\end{bmatrix}  $
\end{figure} 


\begin{figure}[H]
\centering
$J_{OC3}=
\begin{bmatrix}
-\frac{1}{2}s_1l_2    &c_1  &0\\
\frac{1}{2}c_1l_2  & s_1&0\\
0 &0 &0 \\
0 &0 & s1\\
0 &0 &c1\\
1 &0 &0\\
\end{bmatrix}  
$
\end{figure}



\begin{figure}[H]
\centering
$D_1=
\begin{bmatrix}
-\frac{1}{4}(l_2^2m_2)+I_{1YY}    &0  &0\\
0& 0&0\\
0 &0 &0 \\
\end{bmatrix}  
$
\end{figure}


\begin{figure}[H]
\centering
$D_2=
\begin{bmatrix}
\frac{1}{4}(l_2^2c_1^2m_2+l_2^2s_1^2m_2)+I_{2YY}   &0  &0\\
0& m_2&0\\
0 &0 &0 \\
\end{bmatrix}  
$
\end{figure}

\begin{figure}[H]
\centering
$D_3=
\begin{bmatrix}
\frac{1}{4}(l_2^2c_1^2m_3+l_2^2s_1^2m_3)+s^2_3 I_{3XX}+s^2_3 I_{3YY} & 0  & c_3s_3I_{3XX}(c_1^2-s_1^2)+i_{3YY}(c_3s_3s_1^2-c_3^2c_1^2)\\
0& m_3&0\\
I_{3XX}(c_3s_3c_1^2-c_3s_3s_1^2)+I_{3YY}(c_3s_3s_1^2-c_3^2c_1^2) &0 & I_{XX}c_3^2(c_1^2-s_1^2)^2+I_{YY}(c_3c_1^2-s_3s_1^2)^2+I_{3ZZ}(4s_1^2c_1^2)\\
\end{bmatrix}  
$
\end{figure}

\begin{figure}[H]
\centering
$D=D_1+D_2+D_3$
\end{figure}
$
c_{111}=1/2( -1/2 l^2_2 c_1s_1m_2-1/2l_2^2c_1s_1m_2+1/2l_2^2s_1c_1m_2)+1/2( -1/2 l^2_2 c_1 s_1 m_3 -1/2 l_2^2 c_1 s_1 m_3+1/2l_2^2s_1c_1m_3)      \\
c_{113}=I_{3XX}(c_3s_3-2c_1s_1-c_3s_32s_1c_1)+I_{3YY}(c_3s_32s_1c_1+2c_3^2c_1s_1)-s_3c_3I_{3XX}-s_3c_3I_{3YY} \\
c_{133}=1/2(I_{3XX}8c_1s_1(s^2_1-s^2_1)+I_{3YY}(4(c_3+s_3)c_1s_1(s_3s^2_1-c_3s_1^2))+I_{3ZZ}(-8c_1s_1(s^2_1-c_1^2))) \\
c_{333}=1/2(I_{3XX}(-2)s_3c_3(c_1^2-s_1^2)^2)+I_{3YY}(-s_3c_1^2-c_3s_1^2)^2) \\
c_{313}=c_{133} \\
c_{311}=c_{131} \\
c_{131}=c_3s_3(I_{3XX}+I_{3YY}) \\
c_{331}= I_{3XX}(s^2_3-c_3^2)(c_1^2-s_1^2)+I_{3YY}(-s_1^2(s_3^2-c_3^2)-c_3s_3c_1^2)-c_{133} \\

$

\begin{figure}[H]
\centering
$C=
\begin{bmatrix}
 c_{111}\dot{\theta_1^2} + c_{131}\dot{\theta_1}\dot{\theta_3}   +c_{311}\dot{\theta_1}\dot{\theta_3}  \\
 0  \\
 c_{113}\dot{\theta_1^2} + c_{133}\dot{\theta_1}\dot{\theta_3}+c_{333}\dot{\theta_3^2}+c_{313}\dot{\theta_1}\dot{\theta_3}  \\
\end{bmatrix}  
$
\end{figure}






\begin{figure}[H]
\centering
$E_p=E_p_1+E_p_2+E_p_3=m_{1}gl_{1}+m_{2}gl_{1}+m_{3}gl_{1}$

\end{figure}
       
\begin{figure}[H]
\centering
$G=\frac{\delta E_p}{\delta q_k}=\begin{bmatrix}
0\\
0\\
0\\
\end{bmatrix}$
\end{figure}
\begin{figure}[H]
\centering
$
D(q)\dotdot{q} +C(q,\dot{q})+G(q)=\tau
$
\end{figure}







